Add a Fib_Simulate toexperiment compile_generated_files

examples/RoboChart_CSP_sem_basic.thy
@@ -7,8 +7,27 @@ begin
 definition par_hide where
 "par_hide P s Q = (hide (P \<parallel>\<^bsub> s \<^esub> Q) s)"
 
+definition prhide where
+"prhide P es = foldl (\<lambda> Q e. hide Q {e}) P es"
+
 definition discard_state where
 "discard_state P = do {P ; skip}"
+
+(*
+definition "input c = (\<lambda> x. inp c)"
+definition "input_in c A = (\<lambda> x. inp_in c A)"
+
+syntax 
+  "_input"    :: "id \<Rightarrow> pttrn \<Rightarrow> logic \<Rightarrow> logic" ("_?_ \<rightarrow> _" [60, 0, 61] 61)
+  "_input_in" :: "id \<Rightarrow> pttrn \<Rightarrow> logic \<Rightarrow> logic \<Rightarrow> logic" ("_?_:_ \<rightarrow> _" [60, 0, 0, 61] 61)
+  (*"_output"   :: "id \<Rightarrow> logic \<Rightarrow> logic \<Rightarrow> logic" ("_!'(_') \<rightarrow> _" [90, 0, 91] 91)*)
+  "_output"   :: "id \<Rightarrow> logic \<Rightarrow> logic" ("_!'(_')" [90, 0] 91)
+
+translations "c?(x) \<rightarrow> P" == "CONST input c \<Zcomp> (\<lambda> (x). P)"
+translations "c?(x):A \<rightarrow> P" == "CONST input_in c (A) \<Zcomp> (\<lambda> (x). P)"
+(* translations "c!(e) \<rightarrow> P" == "CONST outp c (e) \<Zcomp> P" *)
+translations "c!(e)" == "CONST outp c (e)"
+*)
 
 subsection \<open> General definitions \<close>
 definition "int_max = (2::integer)"
@@ -20,6 +39,15 @@ fun int2integer_list :: "int list \<Rightarrow> integer list" where
 "int2integer_list Nil = Nil" |
 "int2integer_list (Cons x xs) 
   = Cons (integer_of_int x) (int2integer_list xs)"
+
+definition int_to_integer_list :: "int list \<Rightarrow> integer list" where
+"int_to_integer_list = map (integer_of_int)"
+
+lemma "int2integer_list xs = int_to_integer_list xs"
+  apply (simp add: int_to_integer_list_def)
+  apply (induction xs)
+  apply simp
+  by simp
 
 abbreviation "core_int_list \<equiv> 
   int2integer_list [(int_of_integer int_min)..(int_of_integer int_max)]"
@@ -54,7 +82,7 @@ definition "TIDS_stm0_list = [NULLTRANSITION_stm0, TID_stm0_t0, TID_stm0_t1, TID
 definition "TIDS_stm0_set = set TIDS_stm0_list"
 
 definition "ITIDS_stm0_list = [TID_stm0_t1, TID_stm0_t2]"
-definition "ITIDS_stm0 = set ITIDS_stm0_list"
+definition "ITIDS_stm0 = set ITIDS_stm0_list"  
 
 chantype Chan_stm0 =
 (* flow channels *)
@@ -182,6 +210,7 @@ definition stm0_MachineInternalEvents where
 subsubsection \<open> State Machine Memory \<close>
 text \<open> Memory cell processes \<close>
 (* for the shared variable x *)
+
 definition stm0_Memory_opt_x where
 "stm0_Memory_opt_x = 
   loop (\<lambda> s.
@@ -189,6 +218,17 @@ definition stm0_Memory_opt_x where
    do {x \<leftarrow> inp_in set_x_stm0 core_int_set; Ret (x)} \<box>
    do {x \<leftarrow> inp_in set_EXT_x_stm0 core_int_set; Ret (x)})
 )"
+(*
+term "set_x_stm0?(x):(core_int_set) \<rightarrow> (Ret (x))"
+
+definition stm0_Memory_opt_x1 where
+"stm0_Memory_opt_x1 = 
+  loop (\<lambda> s.
+  (do {get_x_stm0!(s) ; Ret (s)}  \<box> 
+   do {set_x_stm0?(x):(core_int_set) \<rightarrow> (Ret (x))} \<box>
+   do {x \<leftarrow> inp_in set_EXT_x_stm0 core_int_set; Ret (x)})
+)"
+*)
 
 (* for the local variable l *)
 definition stm0_Memory_opt_l where
@@ -431,6 +471,415 @@ definition AUX_opt_stm0 where
 definition D__stm0 where
 "D__stm0 (idd::integer) = 
   hide (AUX_opt_stm0 idd) internal_events_stm0
+"
+
+subsection \<open> stm1 \<close>
+
+datatype SIDS_stm1 = SID_stm1
+  | SID_stm1_s0
+
+definition "SIDS_stm1_list = [SID_stm1, SID_stm1_s0]"
+definition "SIDS_stm1_set = set SIDS_stm1_list"
+definition "SIDS_stm1_without_s0 = (removeAll SID_stm1_s0 SIDS_stm1_list)"
+
+datatype TIDS_stm1 = NULLTRANSITION_stm1
+	              | TID_stm1_t0
+	              | TID_stm1_t1
+	              | TID_stm1_t2
+
+definition "TIDS_stm1_list = [NULLTRANSITION_stm1, TID_stm1_t0, TID_stm1_t1, TID_stm1_t2]"
+definition "TIDS_stm1_set = set TIDS_stm1_list"
+
+definition "ITIDS_stm1_list = [TID_stm1_t1, TID_stm1_t2]"
+definition "ITIDS_stm1 = set ITIDS_stm1_list"
+
+chantype Chan_stm1 =
+(* flow channels *)
+  internal_stm1 :: TIDS_stm1
+  enteredV_stm1 :: SIDS_stm1
+  enterV_stm1 :: SIDS_stm1 
+  exitV_stm1  :: SIDS_stm1 
+  exitedV_stm1 :: SIDS_stm1
+  enter_stm1 :: "SIDS_stm1 \<times> SIDS_stm1"
+  entered_stm1 :: "SIDS_stm1 \<times> SIDS_stm1"
+  exit_stm1 :: "SIDS_stm1 \<times> SIDS_stm1"
+  exited_stm1 :: "SIDS_stm1 \<times> SIDS_stm1"
+  terminate_stm1 :: unit (* Is this right? *)
+(* variable channels *)
+  get_l_stm1 :: core_int
+  set_l_stm1 :: core_int
+  get_x_stm1 :: core_int
+  set_x_stm1 :: core_int
+(* shared variable channels *)
+  set_EXT_x_stm1 :: core_int
+(* event channels *)
+  e2__stm1 :: "TIDS_stm1 \<times> InOut"
+  e2_stm1 :: "InOut"
+  e3__stm1 :: "TIDS_stm1 \<times> InOut \<times> core_int"
+  e3_stm1 :: "InOut \<times> core_int"
+
+subsubsection \<open> Sets of events \<close>
+definition int_int_stm1 where
+"int_int_stm1 = 
+  set ([e2__stm1_C (tid, dir). 
+          tid \<leftarrow> [TID_stm1_t1,TID_stm1_t2], 
+          dir \<leftarrow> [din, dout]] @ 
+       [e3__stm1_C (tid, dir, n). 
+          tid \<leftarrow> [TID_stm1_t1,TID_stm1_t2], 
+          dir \<leftarrow> [din, dout], 
+          n \<leftarrow> core_int_list] @
+       [internal_stm1_C (tid). 
+          tid \<leftarrow> [TID_stm1_t1,TID_stm1_t2]]
+)"
+
+definition internal_events_stm1 where
+"internal_events_stm1 = 
+  set ([enter_stm1_C (sid1, sid2). 
+          sid1 \<leftarrow> SIDS_stm1_list, 
+          sid2 \<leftarrow> SIDS_stm1_list] @
+      [entered_stm1_C (sid1, sid2). 
+          sid1 \<leftarrow> SIDS_stm1_list, 
+          sid2 \<leftarrow> SIDS_stm1_list] @
+      [exit_stm1_C (sid1, sid2). 
+          sid1 \<leftarrow> SIDS_stm1_list, 
+          sid2 \<leftarrow> SIDS_stm1_list] @
+      [exited_stm1_C (sid1, sid2). 
+          sid1 \<leftarrow> SIDS_stm1_list, 
+          sid2 \<leftarrow> SIDS_stm1_list]
+)"
+
+definition shared_variable_events_stm1 where
+"shared_variable_events_stm1 = 
+  set ([set_EXT_x_stm1_C (x). 
+          x \<leftarrow> core_int_list]
+)"
+
+definition CS_stm1_s0_sync where
+"CS_stm1_s0_sync = 
+  set ([enter_stm1_C (sidx, sidy). 
+          sidx \<leftarrow> [SID_stm1_s0], 
+          sidy \<leftarrow> [SID_stm1_s0]] @
+      [entered_stm1_C (sidx, sidy). 
+          sidx \<leftarrow> [SID_stm1_s0], 
+          sidy \<leftarrow> [SID_stm1_s0]] @
+      [exit_stm1_C (sidx, sidy). 
+          sidx \<leftarrow> [SID_stm1_s0], 
+          sidy \<leftarrow> [SID_stm1_s0]] @
+      [exited_stm1_C (sidx, sidy). 
+          sidx \<leftarrow> [SID_stm1_s0], 
+          sidy \<leftarrow> [SID_stm1_s0]] @
+      [enter_stm1_C (sidy, sidx). 
+          sidx \<leftarrow> [SID_stm1_s0], 
+          sidy \<leftarrow> [SID_stm1_s0]] @
+      [entered_stm1_C (sidy, sidx). 
+          sidx \<leftarrow> [SID_stm1_s0], 
+          sidy \<leftarrow> [SID_stm1_s0]] @
+      [exit_stm1_C (sidy, sidx). 
+          sidx \<leftarrow> [SID_stm1_s0], 
+          sidy \<leftarrow> [SID_stm1_s0]] @
+      [exited_stm1_C (sidy, sidx). 
+          sidx \<leftarrow> [SID_stm1_s0], 
+          sidy \<leftarrow> [SID_stm1_s0]]
+)"
+
+definition stm1_s0_triggers where
+"stm1_s0_triggers = 
+  set ([e2__stm1_C (tid, dir). 
+          tid \<leftarrow> [TID_stm1_t2], 
+          dir \<leftarrow> [din, dout]] @
+  [e3__stm1_C (tid, dir, n). 
+          tid \<leftarrow> [TID_stm1_t1], 
+          dir \<leftarrow> [din, dout],
+          n \<leftarrow> core_int_list]
+)
+"
+
+definition stm1_l_events where
+"stm1_l_events = 
+    set (
+        [get_l_stm1_C l . l \<leftarrow> core_int_list] @
+        [set_l_stm1_C l . l \<leftarrow> core_int_list]
+    )
+"
+
+definition stm1_x_events where
+"stm1_x_events = 
+    set (
+        [get_x_stm1_C x . x \<leftarrow> core_int_list] @
+        [set_x_stm1_C x . x \<leftarrow> core_int_list] @
+        [set_EXT_x_stm1_C x . x \<leftarrow> core_int_list]
+    )
+"
+
+definition stm1_MachineInternalEvents where
+"stm1_MachineInternalEvents = 
+  set ([internal_stm1_C t . t \<leftarrow> TIDS_stm1_list])
+"
+
+subsubsection \<open> State Machine Memory \<close>
+text \<open> Memory cell processes \<close>
+(* for the shared variable x *)
+
+definition stm1_Memory_opt_x where
+"stm1_Memory_opt_x = 
+  loop (\<lambda> s.
+  (do {outp get_x_stm1 s; Ret (s)} \<box> 
+   do {x \<leftarrow> inp_in set_x_stm1 core_int_set; Ret (x)} \<box>
+   do {x \<leftarrow> inp_in set_EXT_x_stm1 core_int_set; Ret (x)})
+)"
+(*
+term "set_x_stm1?(x):(core_int_set) \<rightarrow> (Ret (x))"
+
+definition stm1_Memory_opt_x1 where
+"stm1_Memory_opt_x1 = 
+  loop (\<lambda> s.
+  (do {get_x_stm1!(s) ; Ret (s)}  \<box> 
+   do {set_x_stm1?(x):(core_int_set) \<rightarrow> (Ret (x))} \<box>
+   do {x \<leftarrow> inp_in set_EXT_x_stm1 core_int_set; Ret (x)})
+)"
+*)
+
+(* for the local variable l *)
+definition stm1_Memory_opt_l where
+"stm1_Memory_opt_l = 
+  loop (\<lambda> s.
+  (do {outp get_l_stm1 s; Ret (s)} \<box> 
+   do {l \<leftarrow> inp_in set_l_stm1 core_int_set; Ret (l)})
+)"
+
+text \<open> Memory transition processes \<close>
+definition stm1_MemoryTransitions_opt_0 where
+"stm1_MemoryTransitions_opt_0 = 
+  loop (\<lambda> id::integer. 
+    (do {outp internal_stm1 TID_stm1_t0 ; Ret (id)} \<box> deadlock)
+  )
+"
+term "do {outp internal_stm1 TID_stm1_t0 ; Ret (id)}"
+term "outp internal_stm1 TID_stm1_t0"
+term "Ret (id)"
+
+definition stm1_MemoryTransitions_opt_1 where
+"stm1_MemoryTransitions_opt_1 = 
+  loop (\<lambda> id::integer.
+    do {x \<leftarrow> inp_in get_x_stm1 core_int_set ; 
+      (
+        do {inp_in e1__stm1 (set [(TID_stm1_t1, din, l). l \<leftarrow> core_int_list, (x = 0)])
+              ; Ret (id)} \<box>
+        do {guard (x \<noteq> 0); outp internal_stm1 TID_stm1_t2 ; Ret (id)} \<box>
+        do {x \<leftarrow> inp_in set_x_stm1 core_int_set; Ret (id)} \<box>
+        do {x \<leftarrow> inp_in set_EXT_x_stm1 core_int_set; Ret (id)}
+      )
+    }
+  )
+"
+
+subsubsection \<open> States \<close>
+definition I_stm1_i0 where
+"I_stm1_i0 = (\<lambda> (id::integer) . 
+  do {outp internal_stm1 TID_stm1_t0 ; 
+      outp set_x_stm1 0; 
+      outp enter_stm1 (SID_stm1, SID_stm1_s0);
+      outp entered_stm1 (SID_stm1, SID_stm1_s0)
+  })
+"
+
+term "(\<lambda> s. Ret (s)) \<Zcomp> (\<lambda> s. Ret (SID_stm1_s0))"
+term "do { Ret (SID_stm1_s0) ; Ret (SID_stm1_s0)}"
+term "do { sd \<leftarrow> inp_in enter_stm1 {(s, SID_stm1_s0) . (s \<in> (SIDS_stm1_set-{SID_stm1_s0}))} ; Ret (snd sd) }"
+term "(\<lambda> s. Ret (s)) \<Zcomp> (\<lambda> s. while (\<lambda> s. fst s) (\<lambda> s. do { Ret (s)}) (s))"
+
+term "(\<lambda> s. do {
+        sd \<leftarrow> inp_in enter_stm1 {(s, SID_stm1_s0) . (s \<in> (SIDS_stm1_set-{SID_stm1_s0}))} ; 
+          Ret (True, idd::integer, fst sd)}) \<Zcomp> 
+          (\<lambda> s. while (\<lambda> s. fst s) (\<lambda> s. 
+            do { Ret (s)}) (s))
+  "
+
+(*
+definition State_stm1_s0 where 
+"State_stm1_s0 = 
+  loop (\<lambda> (id::integer).
+    do {sd \<leftarrow> inp_in enter_stm1 {(s, SID_stm1_s0) . (s \<in> (SIDS_stm1_set-{SID_stm1_s0}))} ; 
+        ret \<leftarrow> Ret (True, id, fst sd) ; 
+        (while (\<lambda> s. fst s) 
+         (\<lambda> s.
+          do {Ret (ret)
+          }) (ret)) ;
+        Ret (id)
+  }
+)
+"
+*)
+
+(* We need an interrupt operator for during actions *) 
+(* ::"integer \<Rightarrow> SIDS_stm1 \<Rightarrow> (Chan_stm1, SIDS_stm1) itree" *)
+definition State_stm1_s0 where 
+"State_stm1_s0 = 
+  loop (\<lambda> (id::integer).
+    do {sd \<leftarrow> inp_in enter_stm1 (set 
+          [(s, SID_stm1_s0) . s \<leftarrow> (removeAll SID_stm1_s0 SIDS_stm1_list)]) ; 
+        \<comment> \<open> State passed to next loop, including a condition initially True. \<close>
+        ret \<leftarrow> Ret (True, id, fst sd) ; 
+        \<comment> \<open> State_stm1_s0_execute \<close>
+        (while 
+           \<comment> \<open> condition \<close>
+           (\<lambda> s. fst s) 
+           \<comment> \<open> P \<close>
+           (\<lambda> s.
+            do {
+              outp entered_stm1 (snd (snd s), SID_stm1_s0);
+                \<comment> \<open> T_stm1_t1 \<close>
+                do {t \<leftarrow> inp_in e1__stm1 (set [(TID_stm1_t1, din, l) . l \<leftarrow> core_int_list]) ;
+                      outp set_l_stm1 (snd (snd t)) ; 
+                      outp exit_stm1 (SID_stm1_s0, SID_stm1_s0);
+                      outp exited_stm1 (SID_stm1_s0, SID_stm1_s0);
+                      l \<leftarrow> inp_in get_l_stm1 core_int_set ; 
+                        outp set_x_stm1 (l);
+                        outp enter_stm1 (SID_stm1_s0, SID_stm1_s0);
+                        Ret(True, fst (snd s), snd (snd s))
+                    } \<box>
+                \<comment> \<open> T_stm1_t2 \<close>
+                do {outp internal_stm1 TID_stm1_t2;
+                    outp exit_stm1 (SID_stm1_s0, SID_stm1_s0);
+                    outp exited_stm1 (SID_stm1_s0, SID_stm1_s0);
+                      x \<leftarrow> inp_in get_x_stm1 core_int_set ; 
+                        outp e3_stm1 (dout, x);
+                        outp enter_stm1 (SID_stm1_s0, SID_stm1_s0);
+                        Ret(True, fst (snd s), snd (snd s))
+                    } \<box>
+                do {
+                    x \<leftarrow> inp_in internal_stm1 
+                      (set (filter (\<lambda> s. s \<in> {NULLTRANSITION_stm1,TID_stm1_t1,TID_stm1_t2}) 
+                          ITIDS_stm1_list));
+                    y \<leftarrow> inp_in exit_stm1 (set 
+                      [(s, SID_stm1_s0) . s \<leftarrow> (removeAll SID_stm1_s0 SIDS_stm1_list)]);
+                      outp exit_stm1 (fst y, SID_stm1_s0);
+                      Ret (False, fst (snd s), snd (snd s))
+                    } \<box>
+                do {
+                    x \<leftarrow> inp_in e1__stm1 (set [(s, d, l) . 
+                        s \<leftarrow> (filter (\<lambda> s. s \<in> {NULLTRANSITION_stm1,TID_stm1_t1,TID_stm1_t2}) 
+                          ITIDS_stm1_list), 
+                        d \<leftarrow> InOut_list,
+                        l \<leftarrow> core_int_list]) ;
+                    y \<leftarrow> inp_in exit_stm1 (set 
+                        [(s, SID_stm1_s0) . s \<leftarrow> (removeAll SID_stm1_s0 SIDS_stm1_list)]);
+                      outp exit_stm1 (fst y, SID_stm1_s0);
+                      Ret (False, fst (snd s), snd (snd s))
+                    } \<box>
+                do {
+                    x \<leftarrow> inp_in e3__stm1 (set [(s, d, l) . 
+                        s \<leftarrow> (filter (\<lambda> s. s \<in> {NULLTRANSITION_stm1,TID_stm1_t1,TID_stm1_t2}) 
+                          ITIDS_stm1_list), 
+                        d \<leftarrow> InOut_list,
+                        l \<leftarrow> core_int_list]) ;
+                    y \<leftarrow> inp_in exit_stm1 (set 
+                        [(s, SID_stm1_s0) . s \<leftarrow> (removeAll SID_stm1_s0 SIDS_stm1_list)]);
+                      outp exit_stm1 (fst y, SID_stm1_s0);
+                      Ret (False, fst (snd s), snd (snd s))
+                    }
+            })
+            \<comment> \<open> The previous state: a triple \<close> 
+            (ret)
+        ) ;
+        Ret (id)
+  }
+)
+"
+
+definition State_stm1_s0_R where
+"State_stm1_s0_R (idd::integer) = 
+   (discard_state (State_stm1_s0 idd)) \<comment> \<open> discard state to match with skip on the right\<close>
+    \<parallel>\<^bsub> (int_int_stm1 - stm1_s0_triggers) \<^esub> 
+   skip
+"
+
+definition STM_stm1 where
+"STM_stm1 (idd::integer) = 
+   (I_stm1_i0(idd))
+    \<parallel>\<^bsub> set (
+        [enter_stm1_C (s, d). 
+          s \<leftarrow> SIDS_stm1_without_s0, 
+          d \<leftarrow> [SID_stm1_s0]] @ 
+        [entered_stm1_C (s, d). 
+          s \<leftarrow> SIDS_stm1_without_s0, 
+          d \<leftarrow> [SID_stm1_s0]] @ 
+        [exit_stm1_C (s, d). 
+          s \<leftarrow> SIDS_stm1_without_s0, 
+          d \<leftarrow> [SID_stm1_s0]] @ 
+        [exited_stm1_C (s, d). 
+          s \<leftarrow> SIDS_stm1_without_s0, 
+          d \<leftarrow> [SID_stm1_s0]] 
+        ) \<^esub> 
+   State_stm1_s0_R(idd)
+"
+
+definition stm1_e1_x_internal_set where
+"stm1_e1_x_internal_set = 
+  set ([e1__stm1_C (tid, dir, n). 
+          tid \<leftarrow> [TID_stm1_t1], 
+          dir \<leftarrow> [din, dout], 
+          n \<leftarrow> core_int_list] @ 
+       [internal_stm1_C TID_stm1_t2] @
+       [set_x_stm1_C n. n \<leftarrow> core_int_list]
+)"
+
+(*
+(Memory_opt_x(0)
+ [| {|set_EXT_x,get_x,set_x|} |] 
+ (
+  (	
+   (
+     ((Memory_opt_l(0) [| {|get_l,set_l|} |] STM_core(id__))\ {|get_l,set_l|})
+     [| {|internal__.TID_stm1_t0|} |]
+     MemoryTransitions_opt_0(id__)
+   ) \ {|internal__.TID_stm1_t0|}
+  )
+  [| {|e1__.TID_stm1_t1,internal__.TID_stm1_t2,set_x|} |]
+  MemoryTransitions_opt_1(id__)
+ )\{|internal__.TID_stm1_t2|}
+) \ {|get_x|}
+*)
+
+subsubsection \<open> State machine \<close>
+definition MemorySTM_opt_stm1 where
+"MemorySTM_opt_stm1 (idd::integer) = 
+  (hide
+    (
+      (discard_state (stm1_Memory_opt_x idd))
+      \<parallel>\<^bsub> stm1_x_events \<^esub>
+      (hide 
+        (
+          (par_hide
+            (par_hide (discard_state (stm1_Memory_opt_l idd)) stm1_l_events (STM_stm1 idd))
+            {internal_stm1_C TID_stm1_t0}
+            (discard_state (stm1_MemoryTransitions_opt_0 idd))
+          )
+          \<parallel>\<^bsub> stm1_e1_x_internal_set \<^esub> 
+          (discard_state (stm1_MemoryTransitions_opt_1 idd))
+        )
+        {internal_stm1_C TID_stm1_t2}
+      )
+    )
+    (set [get_x_stm1_C n. n \<leftarrow> core_int_list])
+  )   
+"
+
+(* Exception: P [| A |> Q*)
+(* Renaming *)
+definition AUX_opt_stm1 where
+"AUX_opt_stm1 (idd::integer) = 
+  (hide 
+    ( 
+      (MemorySTM_opt_stm1 idd)
+    )
+    stm1_MachineInternalEvents
+  )
+"
+
+definition D__stm1 where
+"D__stm1 (idd::integer) = 
+  hide (AUX_opt_stm1 idd) internal_events_stm1
 "
 
 export_code D__stm0 in Haskell 
