examples/Fib_Simulate.thy
@@ -1,0 +1,21 @@
+section \<open>Build and test exported program with MLton\<close>
+
+theory Fib_Simulate
+imports Fib
+begin
+
+(* _ means all generated files in Fib *)
+compile_generated_files
+  _ (in Fib)
+  (* export_files \<open>code/Fib/Fib.hs\<close> *)
+  where \<open>fn dir =>
+    let
+      val exec = Generated_Files.execute 
+        (Path.append (Path.append dir (Path.basic "code")) (Path.basic "Fib"));
+      val cmd = (File.bash_path \<^path>\<open>/usr/bin/ghci\<close> ^
+            " simulate.hs Fib.hs");
+      val log = exec \<open>Simulate\<close> (cmd);
+    in writeln log
+end\<close>
+
+end
